platform/cito/MapSet.v
@@ -1,106 +1,236 @@
-Require Import Memory String.
+Require Import Equalities.
 
 Set Implicit Arguments.
 
-Delimit Scope mapset_scope with mapset.
+Module Type Set_ (Key : MiniDecidableType).
 
-Open Scope mapset.
+  Delimit Scope set_scope with set.
 
-(* PartialMap *)
+  Local Open Scope set_scope.
 
-Variable PartialMap : Set.
+  Parameter set : Type.
 
-Variable sel : PartialMap -> string -> option W.
+  Parameter mem : Key.t -> set -> Prop.
+  Infix "%in" := mem (at level 60): set_scope.
 
-Variable PartialMap_add : PartialMap -> string * W -> PartialMap.
-Infix "%%+" := PartialMap_add (at level 60) : mapset_scope.
+  Parameter union : set -> set -> set.
+  Infix "+" := union : set_scope.
 
-Variable PartialMap_del : PartialMap -> string -> PartialMap.
-Infix "%%-" := PartialMap_del (at level 60) : mapset_scope.
+  Parameter empty : set.
+  Notation "{}" := empty : set_scope.
 
-Hypothesis sel_remove_eq : forall m x, sel (m %%- x) x = None.
+  Parameter singleton : Key.t -> set.
+  Notation "{ x }" := (singleton x) : set_scope.
 
-Hypothesis sel_remove_ne : forall m x x', x <> x' -> sel (m %%- x) x' = sel m x'.
+  Parameter singleton_mem : forall x, mem x {x}.
 
-Hypothesis sel_add_eq : forall m x w, sel (m %%+ (x, w)) x = Some w.
+  Parameter subset : set -> set -> Prop.
+  Infix "<=" := subset : set_scope.
 
-Hypothesis sel_add_ne : forall m x w x', x <> x' -> sel (m %%+ (x, w)) x' = sel m x'.
+  Parameter subset_correct : forall a b, a <= b -> forall x, x %in a -> x %in b.
 
-Variable empty_map : PartialMap.
+  Parameter subset_refl : forall s, s <= s.
 
-Notation "[]" := empty_map : mapset_scope.
+  Parameter subset_union_2 : forall a b, a <= a + b.
 
-Lemma empty_map_empty : forall x, sel [] x = None.
-  admit.
-Qed.
+  Parameter subset_union_1 : forall a b, a <= b + a.
 
-Definition submap (a b : PartialMap) := forall x w, sel a x = Some w -> sel b x = Some w.
+  Parameter union_same_subset : forall s, s + s <= s.
 
-Infix "%%<=" := submap (at level 60) : mapset_scope.
+End Set_.
 
-Lemma submap_correct : forall a b, a %%<= b -> forall x w, sel a x = Some w -> sel b x = Some w.
-  admit.
-Qed.
+Module Type MembershipDecidableSet (Key : MiniDecidableType) <: Set_ Key.
+  
+  Include Set_ Key.
 
-Lemma empty_map_submap : forall m, empty_map %%<= m.
-  admit.
-Qed.
+  Parameter mem_dec : forall x s, {mem x s} + {~ mem x s}.
 
-(* SET *)
+End MembershipDecidableSet.
 
-Variable SET : Set.
+Module Type PartialMap (Key : MiniDecidableType) (Data : Typ).
 
-Variable mem : string -> SET -> Prop.
-Infix "%in" := mem (at level 60): mapset_scope.
+  Delimit Scope pmap_scope with pmap.
 
-Variable union : SET -> SET -> SET.
-Infix "+" := union : mapset_scope.
+  Local Open Scope pmap_scope.
 
-Variable empty_set : SET.
+  Parameter pmap : Type.
 
-Notation "{}" := empty_set : mapset_scope.
+  Parameter sel : pmap -> Key.t -> option Data.t.
 
-Variable singleton_set : string -> SET.
+  Parameter add : pmap -> Key.t * Data.t -> pmap.
+  Infix "+" := add : pmap_scope.
 
-Notation "{ x }" := (singleton_set x) : mapset_scope.
+  Parameter remove : pmap -> Key.t -> pmap.
+  Infix "-" := remove : pmap_scope.
 
-Lemma singleton_mem : forall x, x %in singleton_set x.
-  admit.
-Qed.
+  Parameter sel_remove_eq : forall m x, sel (m - x) x = None.
 
-Variable subset : SET -> SET -> Prop.
+  Parameter sel_remove_ne : forall m x x', x <> x' -> sel (m - x) x' = sel m x'.
 
-Infix "%<=" := subset (at level 60) : mapset_scope.
+  Parameter sel_add_eq : forall m x w, sel (m + (x, w)) x = Some w.
 
-Lemma subset_correct : forall a b, a %<= b -> forall x, x %in a -> x %in b.
-  admit.
-Qed.
+  Parameter sel_add_ne : forall m x w x', x <> x' -> sel (m + (x, w)) x' = sel m x'.
 
-Lemma subset_union_2 : forall a b, a %<= a + b.
-  admit.
-Qed.
+  Parameter empty : pmap.
+  Notation "[]" := empty : pmap_scope.
 
-Lemma subset_union_1 : forall a b, a %<= b + a.
-  admit.
-Qed.
+  Parameter empty_correct : forall x, sel [] x = None.
 
-Lemma subset_refl : forall s, s %<= s.
-  admit.
-Qed.
+End PartialMap.
 
-Lemma union_same_subset : forall s, s + s %<= s.
-  admit.
-Qed.
+Module Type HasSubtract (Key : MiniDecidableType) (Data : Typ) (S : Set_ Key) <: PartialMap Key Data.
 
-(* subtract *)
+  Include PartialMap Key Data.
 
-Variable subtract : PartialMap -> SET -> PartialMap.
-Infix "-" := subtract : mapset_scope.
+  Local Open Scope pmap_scope.
 
-Lemma subtract_submap : forall a b, a - b %%<= a.
-  admit.
-Qed.
+  Parameter subtract : pmap -> S.set -> pmap.
+  Infix "--" := subtract (at level 60) : pmap_scope.
 
-Lemma subtract_none : forall m s x, x %in s -> sel (m - s) x = None.
-  admit.
-Qed.
+  Parameter subtract_none : forall m s x, S.mem x s -> sel (m -- s) x = None.
+
+  Parameter subtract_in : forall m s x w, sel (m -- s) x = Some w -> sel m x = Some w.
+
+End HasSubtract.
+
+(* Implementations *)
+
+Module ArrowSet (Key : MiniDecidableType) : MembershipDecidableSet Key.
+
+  Definition set := Key.t -> bool.
+
+  Definition mem x (s : set) := s x = true.
+
+  Definition union (a b : set) := fun x => orb (a x) (b x).
+
+  Definition empty : set := fun _ => false.
+
+  Definition singleton a : set := fun x => if Key.eq_dec x a then true else false.
+
+  Lemma singleton_mem : forall x, mem x (singleton x).
+    unfold singleton, mem; intros; destruct (Key.eq_dec x x); eauto.
+  Qed.
+
+  Definition subset (a b : set) := forall x, mem x a -> mem x b.
+
+  Lemma subset_correct : forall a b, subset a b -> forall x, mem x a -> mem x b.
+    eauto.
+  Qed.
+
+  Definition subset_refl : forall s, subset s s.
+    unfold subset; intuition.
+  Qed.
+
+  Definition subset_union_2 : forall a b, subset a (union a b).
+    unfold subset, union, mem; intuition.
+  Qed.
+  
+  Definition subset_union_1 : forall a b, subset a (union b a).
+    unfold subset, union, mem; intuition.
+  Qed.
+
+  Definition union_same_subset : forall s, subset (union s s) s.
+    unfold subset, union, mem; intuition.
+    eapply Bool.orb_true_elim in H.
+    destruct H; eauto.
+  Qed.
+
+  Definition mem_dec : forall x s, {mem x s} + {~ mem x s}.
+    unfold mem; intros; destruct (Bool.bool_dec (s x) true); intuition.
+  Qed.
+
+End ArrowSet.
+
+Module ArrowPMap (Key : MiniDecidableType) (Data : Typ) <: PartialMap Key Data.
+
+  Definition pmap := Key.t -> option Data.t.
+
+  Definition sel (m : pmap) := m.
+
+  Definition add (m : pmap) (p : Key.t * Data.t) : pmap :=
+    fun k =>
+      if Key.eq_dec k (fst p) then
+        Some (snd p)
+      else
+        m k.
+
+  Definition remove (m : pmap) (k : Key.t) : pmap :=
+    fun k' =>
+      if Key.eq_dec k' k then
+        None
+      else
+        m k'.
+
+  Lemma sel_remove_eq : forall m x, sel (remove m x) x = None.
+    unfold sel, remove; intros; destruct (Key.eq_dec x x); intuition.
+  Qed.
+    
+  Lemma sel_remove_ne : forall m x x', x <> x' -> sel (remove m x) x' = sel m x'.
+    unfold sel, remove; intros; destruct (Key.eq_dec x' x); subst; intuition.
+  Qed.
+
+  Lemma sel_add_eq : forall m x w, sel (add m (x, w)) x = Some w.
+    unfold sel, add; simpl; intros; destruct (Key.eq_dec x x); intuition.
+  Qed.
+
+  Lemma sel_add_ne : forall m x w x', x <> x' -> sel (add m (x, w)) x' = sel m x'.
+    unfold sel, add; simpl; intros; destruct (Key.eq_dec x' x); subst; intuition.
+  Qed.
+
+  Definition empty : pmap := fun _ => None.
+
+  Lemma empty_correct : forall x, sel empty x = None.
+    eauto.
+  Qed.
+
+End ArrowPMap.
+
+Module ArrowHasSubtract (Key : MiniDecidableType) (Data : Typ) (S : MembershipDecidableSet Key) <: HasSubtract Key Data S.
+
+  Include ArrowPMap Key Data.
+
+  Definition subtract (m : pmap) (s : S.set) : pmap :=
+    fun k =>
+      if S.mem_dec k s then
+        None
+      else
+        sel m k.
+
+  Lemma subtract_none : forall m s x, S.mem x s -> sel (subtract m s) x = None.
+    unfold subtract, sel; intros; destruct (S.mem_dec x s); intuition.
+  Qed.
+
+  Lemma subtract_in : forall m s x w, sel (subtract m s) x = Some w -> sel m x = Some w.
+    unfold subtract, sel; intros; destruct (S.mem_dec x s); intuition; discriminate.
+  Qed.
+
+End ArrowHasSubtract.
+
+Module MakeSubmap (Key : MiniDecidableType) (Data : Typ) (M : PartialMap Key Data) <: PartialMap Key Data.
+
+  Include M.
+
+  Definition submap (a b : pmap) := forall x w, sel a x = Some w -> sel b x = Some w.
+  Infix "<=" := submap : pmap_scope.
+
+  Lemma submap_correct : forall a b, submap a b -> forall x w, sel a x = Some w -> sel b x = Some w.
+    eauto.
+  Qed.
+
+  Lemma empty_submap : forall m, submap empty m.
+    unfold submap; intros; rewrite empty_correct in H; discriminate.
+  Qed.
+
+End MakeSubmap.
+
+Module SubtractSubmap (Key : MiniDecidableType) (Data : Typ) (S : MembershipDecidableSet Key) (M : HasSubtract Key Data S) <: HasSubtract Key Data S.
+
+  Include M.
+
+  Module Submap := MakeSubmap Key Data M.
+
+  Lemma subtract_submap : forall (a : pmap) (b : S.set), Submap.submap (subtract a b) a.
+    unfold Submap.submap; intros; eapply subtract_in; eauto.
+  Qed.
+
+End SubtractSubmap.
